Dafny/examples/BasicBug/simpleBugBenignLemmas.i.dfy
@@ -1,0 +1,154 @@
+include "simpleBugCode.i.dfy"
+include "simpleBugGeneral.i.dfy"
+include "../../LLVM/llvmREFACTOR.i.dfy"
+include "../../LLVM/types.dfy"
+
+module simpleBugBenignLemmas{
+    import opened simpleBugCode
+    import opened simpleBugGeneral
+    import opened LLVM_defRE
+    import opened types
+
+
+    lemma possibleVulnOutputs(s:state, b:behavior) 
+        requires ValidState(s);
+        requires |b| > 0;
+        requires b[0] == s;
+        requires s.o.Nil?;
+
+        ensures  forall input :: (validInput(s,input) && OperandContents(s,input).val < 2 && BehaviorEvalsCode(codeVuln(input),b)) 
+                                  ==> (behaviorOutput(b) == [Nil,Nil,Nil,Out((Int(1,IntType(1,false)))),Out((Int(1,IntType(1,false))))]);
+        ensures  forall input :: (validInput(s,input) && OperandContents(s,input).val >= 2 && BehaviorEvalsCode(codeVuln(input),b)) 
+                                  ==> (behaviorOutput(b) == [Nil,Nil,Nil,Out((Int(0,IntType(1,false)))),Out((Int(0,IntType(1,false))))]);
+    {
+        var inputWitness := D(Int(1,IntType(4,false)));
+        assert validInput(s,inputWitness);
+        forall input | validInput(s,input) && OperandContents(s,input).val < 2 && BehaviorEvalsCode(codeVuln(input),b)
+            ensures (behaviorOutput(b) == [Nil,Nil,Nil,Out((Int(1,IntType(1,false)))),Out((Int(1,IntType(1,false))))]);
+        {
+            var input :| validInput(s,input) && OperandContents(s,input).val < 2 && BehaviorEvalsCode(codeVuln(input),b);
+            var b' := unwrapVulnBehaviors(s,input);
+        }
+        forall input | validInput(s,input) && OperandContents(s,input).val >= 2 && BehaviorEvalsCode(codeVuln(input),b)
+            ensures (behaviorOutput(b) == [Nil,Nil,Nil,Out((Int(0,IntType(1,false)))),Out((Int(0,IntType(1,false))))]);
+        {
+            var input :| validInput(s,input) && OperandContents(s,input).val >= 2 && BehaviorEvalsCode(codeVuln(input),b);
+            var b' := unwrapVulnBehaviors(s,input);
+        }
+     
+    }
+
+    lemma vulnBehaviorIncludesPatchedBehavior(s:state,b:behavior,vulnBehaviors:seq<behavior>)
+        requires ValidState(s);
+        requires validPatchBehavior(b)
+        requires |b| > 0;
+        requires |vulnBehaviors| > 0; 
+        requires b[0] == s;
+        requires forall v :: v in vulnBehaviors <==> (exists input :: validInput(s,input) && BehaviorEvalsCode(codeVuln(input),v) && v[0] == s)
+        ensures exists v :: (v in vulnBehaviors && equalOutput(behaviorOutput(v), [Nil,Nil,Nil,Out((Int(1,IntType(1,false)))),Out((Int(1,IntType(1,false))))]));
+        // ensures  [Nil,Nil,Nil,Out((Int(1,IntType(1,false)))),Out((Int(1,IntType(1,false))))] in allBehaviorOutput(vulnBehaviors);
+
+    {
+        validInputVulnImpliesBehavior(s);
+        var input :| BehaviorEvalsCode(codePatch(input),b) && |b| > 0 && validInput(b[0],input);
+        var b' := unwrapPatchBehaviors(s,input);
+        // assert equalOutput(behaviorOutput(b),[Nil,Nil,Nil,Out((Int(1,IntType(1,false)))),Out((Int(1,IntType(1,false))))]);
+        // equalOutputLemma(behaviorOutput(b),[Nil,Nil,Nil,Out((Int(1,IntType(1,false)))),Out((Int(1,IntType(1,false))))]);
+        assert exists vuln, vulnIn :: vuln in vulnBehaviors && validInput(s,vulnIn)  && OperandContents(s,vulnIn).val < 2 && BehaviorEvalsCode(codeVuln(vulnIn),vuln);
+        var vuln, vulnIn :| vuln in vulnBehaviors && validInput(s,vulnIn)  && OperandContents(s,vulnIn).val < 2 && BehaviorEvalsCode(codeVuln(vulnIn),vuln);
+        possibleVulnOutputs(s,vuln);
+        assert equalOutput(behaviorOutput(vuln),[Nil,Nil,Nil,Out((Int(1,IntType(1,false)))),Out((Int(1,IntType(1,false))))]);
+        
+        assert vuln in vulnBehaviors && equalOutput(behaviorOutput(vuln), behaviorOutput(b));
+        assert exists v :: (v in vulnBehaviors && equalOutput(behaviorOutput(v), behaviorOutput(b)));
+        var vulnOut := allBehaviorOutput(vulnBehaviors);
+        assert forall v :: v in vulnBehaviors ==> behaviorOutput(v) in vulnOut;
+        assert [Nil,Nil,Nil,Out((Int(1,IntType(1,false)))),Out((Int(1,IntType(1,false))))] in vulnOut;
+
+    }
+
+
+    lemma patchIsBenignTrivial(s:state,vulnBehaviors:seq<behavior>,patchBehaviors:seq<behavior>,vulnOut:seq<seq<output>>,patchOut:seq<seq<output>>)
+        requires |patchBehaviors| == 0
+        requires |patchOut| == 0
+        requires ValidState(s);
+        requires forall b :: b in vulnBehaviors <==> (exists input :: validInput(s,input) && BehaviorEvalsCode(codeVuln(input),b) && b[0] == s)
+        requires forall b :: b in patchBehaviors <==> (exists input :: validInput(s,input) && BehaviorEvalsCode(codePatch(input),b) && b[0] == s)
+
+        ensures forall p :: p in patchOut ==> p in vulnOut
+        {
+           
+            assert |patchBehaviors| == 0;
+            assert |patchOut| == 0;
+            assert forall p :: p in patchBehaviors ==> p in vulnBehaviors;
+            assert forall p :: p in patchBehaviors ==> (exists v :: v in vulnBehaviors && equalOutput(behaviorOutput(v), behaviorOutput(p)));
+            assert forall p :: p in patchOut ==> p in vulnOut;
+            
+        }
+
+
+    lemma patchIsBenignNonTrivial(s:state,vulnBehaviors:seq<behavior>,patchBehaviors:seq<behavior>,vulnOut:seq<seq<output>>,patchOut:seq<seq<output>>)
+        requires nonTrivialBehaviorPreconditions(s,vulnBehaviors,patchBehaviors)
+        requires |patchBehaviors| > 0;
+        requires vulnOut == allBehaviorOutput(vulnBehaviors);
+        requires patchOut ==  allBehaviorOutput(patchBehaviors);
+
+        ensures forall p :: p in patchBehaviors ==> exists v :: (v in vulnBehaviors && equalOutput(behaviorOutput(v), behaviorOutput(p)));
+        ensures forall p :: p in patchBehaviors ==> equalOutput(behaviorOutput(p),[Nil,Nil,Nil,Out((Int(1,IntType(1,false)))),Out((Int(1,IntType(1,false))))]);
+        ensures forall p :: p in patchBehaviors ==> behaviorOutput(p) in vulnOut;
+        ensures forall p :: p in patchBehaviors ==> behaviorOutput(p) in patchOut;
+    {
+        validInputVulnImpliesBehavior(s);
+        assert |patchBehaviors| > 0;
+        assert forall p :: p in patchBehaviors ==> validPatchBehavior(p);
+        // assert forall x :: x in allBehaviors(patchBehaviors) ==> equalOutput(x,[Nil,Nil,Nil,Out((Int(1,IntType(1,false)))),Out((Int(1,IntType(1,false))))]);
+        forall p | p in patchBehaviors
+            ensures exists v :: (v in vulnBehaviors && equalOutput(behaviorOutput(v), behaviorOutput(p)));
+            ensures equalOutput(behaviorOutput(p),[Nil,Nil,Nil,Out((Int(1,IntType(1,false)))),Out((Int(1,IntType(1,false))))]);
+            ensures behaviorOutput(p) in vulnOut;
+            ensures behaviorOutput(p) in patchOut;
+            {
+
+                var input :| BehaviorEvalsCode(codePatch(input),p) && |p| > 0 && validInput(p[0],input);
+                var b' := unwrapPatchBehaviors(s,input);
+                assert equalOutput(behaviorOutput(p),[Nil,Nil,Nil,Out((Int(1,IntType(1,false)))),Out((Int(1,IntType(1,false))))]);
+
+                vulnBehaviorIncludesPatchedBehavior(s,p,vulnBehaviors);
+                assert exists v :: (v in vulnBehaviors && equalOutput(behaviorOutput(v), [Nil,Nil,Nil,Out((Int(1,IntType(1,false)))),Out((Int(1,IntType(1,false))))]));
+                var v :| (v in vulnBehaviors && equalOutput(behaviorOutput(v), [Nil,Nil,Nil,Out((Int(1,IntType(1,false)))),Out((Int(1,IntType(1,false))))]));
+                assert behaviorOutput(v) in vulnOut;
+                
+                transitiveEquality(behaviorOutput(p),behaviorOutput(v),[Nil,Nil,Nil,Out((Int(1,IntType(1,false)))),Out((Int(1,IntType(1,false))))]);
+                assert behaviorOutput(p) == behaviorOutput(v);
+                equalOutputIsTransitive(behaviorOutput(v),behaviorOutput(p),vulnOut);
+                assert behaviorOutput(p) in vulnOut;
+            }
+            
+    }
+
+   lemma validInputPatchImpliesBehavior(s:state)
+        requires ValidState(s);
+        ensures forall input :: validInput(s,input) ==> (exists b :: BehaviorEvalsCode(codePatch(input),b) && b[0] == s)
+    {
+        forall input | validInput(s,input)
+            ensures exists b :: BehaviorEvalsCode(codePatch(input),b) && b[0] == s
+        {
+            var b := unwrapPatchBehaviors(s,input);
+            assert exists b' :: BehaviorEvalsCode(codePatch(input),b') && b'[0] == s;
+        }
+    }
+
+    lemma validInputVulnImpliesBehavior(s:state)
+        requires ValidState(s);
+        ensures forall input :: validInput(s,input) ==> (exists b :: BehaviorEvalsCode(codeVuln(input),b) && b[0] == s)
+    {
+        forall input | validInput(s,input)
+            ensures exists b :: BehaviorEvalsCode(codeVuln(input),b) && b[0] == s
+        {
+            var b := unwrapVulnBehaviors(s,input);
+            assert exists b' :: BehaviorEvalsCode(codeVuln(input),b') && b'[0] == s;
+        }
+    }
+
+    
+}
