Dafny/examples/BasicBug/simpleBugCode.i.dfy
@@ -1,0 +1,428 @@
+include "../../LLVM/llvmREFACTOR.i.dfy"
+include "../../LLVM/types.dfy"
+include "../../Libraries/Seqs.s.dfy"
+include "../../LLVM/Operations/binaryOperations.i.dfy"
+
+module simpleBugCode{
+
+    import opened types
+    import opened LLVM_defRE
+    import opened binary_operations_i
+    import opened Collections__Seqs_s
+
+// c function //
+// int testOverflow(int x)
+// {
+//   if (x < 0 || x > 2){
+//     return -2;
+//   }
+//   int y = INT_MAX-1;
+//   int z = x + y;
+//   if(z > 0){
+//     return 42;
+//   }else{
+//     return -1;
+//   }
+
+// ---------------------------------------------------
+// -03
+// ; Function Attrs: nofree norecurse nosync nounwind readnone uwtable willreturn mustprogress
+// define dso_local i32 @testOverflow(i32 %x) local_unnamed_addr #2 {
+// entry:
+//   %0 = icmp ugt i32 %x, 2
+//   %retval.1 = select i1 %0, i32 -2, i32 42
+//   ret i32 %retval.1
+// }
+// ---------------------------------------------------
+// No Opt
+// ; Function Attrs: noinline nounwind optnone uwtable
+// define dso_local i32 @testOverflow(i32 %x) #0 {
+// entry:
+//   %retval = alloca i32, align 4
+//   %x.addr = alloca i32, align 4
+//   %y = alloca i32, align 4
+//   %z = alloca i32, align 4
+//   store i32 %x, i32* %x.addr, align 4
+//   %0 = load i32, i32* %x.addr, align 4
+//   %cmp = icmp slt i32 %0, 0
+//   br i1 %cmp, label %if.then, label %lor.lhs.false
+
+// lor.lhs.false:                                    ; preds = %entry
+//   %1 = load i32, i32* %x.addr, align 4
+//   %cmp1 = icmp sgt i32 %1, 2
+//   br i1 %cmp1, label %if.then, label %if.end
+
+// if.then:                                          ; preds = %lor.lhs.false, %entry
+//   store i32 -2, i32* %retval, align 4
+//   br label %return
+
+// if.end:                                           ; preds = %lor.lhs.false
+//   store i32 2147483646, i32* %y, align 4
+//   %2 = load i32, i32* %x.addr, align 4
+//   %3 = load i32, i32* %y, align 4
+//   %add = add nsw i32 %2, %3
+//   store i32 %add, i32* %z, align 4
+//   %4 = load i32, i32* %z, align 4
+//   %cmp2 = icmp sgt i32 %4, 0
+//   br i1 %cmp2, label %if.then3, label %if.else
+
+// if.then3:                                         ; preds = %if.end
+//   store i32 42, i32* %retval, align 4
+//   br label %return
+
+// if.else:                                          ; preds = %if.end
+//   store i32 -1, i32* %retval, align 4
+//   br label %return
+
+// return:                                           ; preds = %if.else, %if.then3, %if.then
+//   %5 = load i32, i32* %retval, align 4
+//   ret i32 %5
+// }
+// ---------------------------------------------------
+// Mixed
+// ; Function Attrs: nofree norecurse nosync nounwind readnone uwtable willreturn mustprogress
+// define dso_local i32 @testOverflow(i32 %x) local_unnamed_addr #2 {
+// entry:
+    // %cmp = icmp slt i32 %x, 0
+
+
+
+    predicate validInput(s:state, input:operand)
+        requires ValidState(s)
+    {
+        // var result := LV("result");
+        && s.o.Nil?
+        && ValidOperand(s,input)
+        && isInt(OperandContents(s,input))
+        && typesMatch(OperandContents(s,D(Int(0,IntType(4,false)))),OperandContents(s,input))
+        && OperandContents(s,input).val >= 0 
+        && OperandContents(s,input).val <= 2
+        // && ValidOperand(s,result)
+    }
+
+
+    function codeVuln(x:operand):codeRe
+    {
+        var z := LV("z");
+        var result := LV("result");
+
+        var y := D(Int(2147483646,IntType(4,false)));
+
+        var cSeq := [Ins(ADD(z,4,x,y)),
+                     Ins(ICMP(result,sgt,4,z,D(Int(0,IntType(4,false))))),
+                     Ins(RET(result))];
+        Block(cSeq)
+    }
+    
+    function codePatch(x:operand):codeRe
+    {
+        var z := LV("z");
+        var result := LV("result");
+
+        var y := D(Int(2147483646,IntType(4,false)));
+
+        var cSeq := [Ins(ADD(z,4,x,y)),
+                     Ins(ICMP(result,ugt,4,z,D(Int(0,IntType(4,false))))),
+                     Ins(RET(result))];
+        Block(cSeq)
+    }
+
+
+    lemma unwrapPatchBehaviors(s:state, input:operand) returns (b:behavior)
+        requires ValidState(s);
+
+        // -- input is valid -- ie. valid 16 bit integer 
+        requires validInput(s,input);
+        ensures |b| == 5;
+        ensures b[0] == s;
+        ensures forall i :: i > 0 && i < |b|-1 ==> b[i] == evalInsRe(codePatch(input).block[i-1].ins,b[i-1]);
+        ensures b[|b|-1] == b[|b|-2];
+        // ensures b == [s] + evalCodeRE(c,s)
+
+
+        ensures ValidBehaviorNonTrivial(b);
+        ensures BehaviorEvalsCode(codePatch(input),b);
+
+
+        ensures ValidBehaviorNonTrivial(b);
+        ensures BehaviorEvalsCode(codePatch(input),b);
+        ensures forall b' :: (BehaviorEvalsCode(codePatch(input),b')  && b'[0] == b[0]) ==> b' == b
+
+        ensures exists patch :: BehaviorEvalsCode(codePatch(input),patch) && b == patch;
+        // ensures  exists result :: (
+        //                 && ValidOperand(last(b),result)
+        //                 && OperandContents(last(b),result).Int?
+        //                 && OperandContents(last(b),result).val == 1);
+        ensures (behaviorOutput(b) == [Nil,Nil,Nil,Out((Int(1,IntType(1,false)))),Out((Int(1,IntType(1,false))))]);
+
+        {
+            var c := codePatch(input);
+            assert forall cs :: cs in c.block ==> !cs.CNil?;
+            assert |c.block| == 3;
+            b := [s] + evalCodeRE(c,s);
+            
+            var step,remainder, subBehavior := unwrapBlockWitness(b,c.block,s);
+
+            step,remainder,subBehavior := unwrapBlockWitness(subBehavior,remainder,last(step));
+            step,remainder,subBehavior := unwrapBlockWitness(subBehavior,remainder,last(step));
+            step,remainder,subBehavior := unwrapBlockWitness(subBehavior,remainder,last(step));
+  
+            var z := LV("z");
+            var result := LV("result");
+            
+            var y := D(Int(2147483646,IntType(4,false)));
+
+
+            assert c == Block([Ins(ADD(z,4,input,y)),
+                            Ins(ICMP(result,ugt,4,z,D(Int(0,IntType(4,false))))),
+                            Ins(RET(result))]);
+
+
+            assert b[0] == s;
+            assert b[1] == evalInsRe(ADD(z,4,input,y),s);
+            
+            // ADD
+            assert ValidInstruction(s,ADD(z,4,input,y));
+            assert NextStep(s,b[1], Step.evalInsStep(ADD(z,4,input,y))); 
+            assert StateNext(b[0],b[1]);
+            assert ValidState(b[1]);
+            assert b[1] == stateUpdateVar(s,z,evalADD(4,OperandContents(s,D(Int(2147483646,IntType(4,false)))),OperandContents(s,input)));
+            assert OperandContents(b[1],z).Int?;
+            assert ToTwosComp(OperandContents(b[1],z)).val == (Int(2147483646,IntType(4,false)).val + OperandContents(s,input).val) % Pow256(4); 
+            assert OperandContents(s,input).val > 0 ==> OperandContents(b[1],z).val > 0;
+        
+            // ICMP
+            assert ValidOperand(b[1],z);
+            assert ValidOperand(b[1],D(Int(0,IntType(4,false))));
+            assert isInt(OperandContents(b[1],z)) && isInt(OperandContents(b[1],D(Int(0,IntType(4,false)))));
+            assert typesMatch(OperandContents(b[1],z),OperandContents(b[1],D(Int(0,IntType(4,false)))));
+            assert 4 == OperandContents(b[1],z).itype.size;
+            assert ValidInstruction(b[1],ICMP(result,ugt,4,z,D(Int(0,IntType(4,false)))));
+            assert NextStep(b[1],b[2],Step.evalInsStep(ICMP(result,ugt,4,z,D(Int(0,IntType(4,false))))));
+            assert StateNext(b[1],b[2]);
+            assert ValidState(b[2]);
+    //
+            assert ValidOperand(b[2],result);
+            assert OperandContents(b[2],result).Int?;
+            assert OperandContents(b[2],result).val == 1;
+            assert ValidInstruction(b[2],RET(result));
+            assert NextStep(b[2],b[3],Step.evalInsStep(RET(result)));
+            assert StateNext(b[2],b[3]);
+            assert OperandContents(b[2],result) == OperandContents(b[3],result);
+            assert ValidState(b[3]);
+
+            // LAST STEP
+            assert b[3] == b[4];
+            assert ValidState(b[4]);
+            assert NextStep(b[3],b[4],Step.stutterStep());
+            assert StateNext(b[3],b[4]);
+            
+            // Properties
+            assert ValidBehaviorNonTrivial(b);
+            assert BehaviorEvalsCode(c,b);
+            assert OperandContents(b[1],z).val > 0 ==> OperandContents(b[2],result).val == 1;
+            assert ValidOperand(last(b),z);
+            assert OperandContents(s,input).val > 0 ==> OperandContents(b[1],z).val > 0;
+            assert |b| == 5;
+            // assert forall b' :: (b' in b && ValidOperand(b',result) && OperandContents(b',result).Int?) ==> OperandContents(b',result).val != 0;
+            assert Out(OperandContents(b[2],result)) in behaviorOutput(b);
+            assert OperandContents(b[2],result) == (Int(1,IntType(1,false)));
+            // assert OperandContents(b[2],result) == (Int(1,IntType(1,false)));
+            assert behaviorOutput(b) == [Nil,Nil,Nil,Out((Int(1,IntType(1,false)))),Out((Int(1,IntType(1,false))))];
+            // outputIsEqual(behaviorOutput(b) , [Nil,Nil,Nil,Out(OperandContents(b[2],result)),Out(OperandContents(b[2],result))]);
+         
+            assert OperandContents(last(b),result).val == 1;
+            uniqueOperandContent(last(b),result);
+            assert !(OperandContents(last(b),result).val == 0);
+            uniqueOperandInState(last(b),result);
+            // assert (exists s:state :: (s == last(b) && s in b 
+            //                   && ValidState(s)
+            //                   && ValidOperand(s,result)
+            //                   && OperandContents(s,result).Int?
+            //                   && OperandContents(s,result).val == 1));
+
+            // assert (exists s:state,result:operand :: (&& s in b
+            //                                         && last(b) == s 
+            //                                         && ValidState(s)
+            //                                         && result.LV?
+            //                                         && result.l in s.lvs
+            //                                         && ValidOperand(s,result)
+            //                                         && OperandContents(s,result).Int?
+            //                                         && OperandContents(s,result).val == 1));
+
+
+        }
+
+     lemma unwrapVulnBehaviors(s:state, input:operand) returns (b:behavior)
+        requires ValidState(s);
+
+        // -- input is valid -- ie. valid 16 bit integer 
+        requires validInput(s,input);
+        ensures |b| == 5;
+        ensures b[0] == s;
+        ensures forall i :: i > 0 && i < |b|-1 ==> b[i] == evalInsRe(codeVuln(input).block[i-1].ins,b[i-1]);
+        ensures b[|b|-1] == b[|b|-2];
+        // ensures b == [s] + evalCodeRE(c,s)
+
+
+        ensures ValidBehaviorNonTrivial(b);
+        ensures BehaviorEvalsCode(codeVuln(input),b);
+        ensures forall b' :: (BehaviorEvalsCode(codeVuln(input),b')  && b'[0] == b[0]) ==> b' == b
+
+        ensures exists input :: validInput(s,input) && BehaviorEvalsCode(codeVuln(input),b) && b[0] == s
+
+        ensures ValidBehaviorNonTrivial(b);
+        ensures BehaviorEvalsCode(codeVuln(input),b);
+        ensures (behaviorOutput(b) == [Nil,Nil,Nil,Out((Int(1,IntType(1,false)))),Out((Int(1,IntType(1,false))))])
+                || (behaviorOutput(b) == [Nil,Nil,Nil,Out((Int(0,IntType(1,false)))),Out((Int(0,IntType(1,false))))]);
+        ensures (OperandContents(s,input).val < 2) ==> (behaviorOutput(b) == [Nil,Nil,Nil,Out((Int(1,IntType(1,false)))),Out((Int(1,IntType(1,false))))]);
+        ensures (OperandContents(s,input).val >= 2) ==> (behaviorOutput(b) == [Nil,Nil,Nil,Out((Int(0,IntType(1,false)))),Out((Int(0,IntType(1,false))))]);
+         ensures OperandContents(s,input).val == 2 ==>( exists result:operand :: 
+                                                            (&& ValidState(last(b))
+                                                            && result.LV?
+                                                            && result.l in last(b).lvs
+                                                            && ValidOperand(last(b),result)
+                                                            && OperandContents(last(b),result).Int?
+                                                            && OperandContents(last(b),result).val == 0));
+        {
+            var c := codeVuln(input);
+            assert forall cs :: cs in c.block ==> !cs.CNil?;
+            assert |c.block| == 3;
+            b := [s] + evalCodeRE(c,s);
+            
+            var step,remainder, subBehavior := unwrapBlockWitness(b,c.block,s);
+
+            step,remainder,subBehavior := unwrapBlockWitness(subBehavior,remainder,last(step));
+            step,remainder,subBehavior := unwrapBlockWitness(subBehavior,remainder,last(step));
+            step,remainder,subBehavior := unwrapBlockWitness(subBehavior,remainder,last(step));
+  
+            var z := LV("z");
+            var result := LV("result");
+            var y := D(Int(2147483646,IntType(4,false)));
+
+
+            assert c == Block([Ins(ADD(z,4,input,y)),
+                            Ins(ICMP(result,sgt,4,z,D(Int(0,IntType(4,false))))),
+                            Ins(RET(result))]);
+
+
+            assert b[0] == s;
+            assert b[1] == evalInsRe(ADD(z,4,input,y),s);
+            
+            // ADD
+            assert ValidInstruction(s,ADD(z,4,input,y));
+            assert NextStep(s,b[1], Step.evalInsStep(ADD(z,4,input,y))); 
+            assert StateNext(b[0],b[1]);
+            assert ValidState(b[1]);
+            assert b[1] == stateUpdateVar(s,z,evalADD(4,OperandContents(s,D(Int(2147483646,IntType(4,false)))),OperandContents(s,input)));
+            assert OperandContents(b[1],z).Int?;
+            assert ToTwosComp(OperandContents(b[1],z)).val == (Int(2147483646,IntType(4,false)).val + OperandContents(s,input).val) % Pow256(4);
+            assert OperandContents(s,input).val == 2 ==>   OperandContents(b[1],z).val == 2147483648;
+            assert OperandContents(s,input).val == 2 ==>  FromTwosComp(OperandContents(b[1],z)).val < 0;
+            assert OperandContents(s,input).val > 0 ==> OperandContents(b[1],z).val > 0;
+        
+            // ICMP
+            assert ValidOperand(b[1],z);
+            assert ValidOperand(b[1],D(Int(0,IntType(4,false))));
+            assert isInt(OperandContents(b[1],z)) && isInt(OperandContents(b[1],D(Int(0,IntType(4,false)))));
+            assert typesMatch(OperandContents(b[1],z),OperandContents(b[1],D(Int(0,IntType(4,false)))));
+            assert 4 == OperandContents(b[1],z).itype.size;
+            assert ValidInstruction(b[1],ICMP(result,sgt,4,z,D(Int(0,IntType(4,false)))));
+            assert NextStep(b[1],b[2],Step.evalInsStep(ICMP(result,sgt,4,z,D(Int(0,IntType(4,false))))));
+            assert StateNext(b[1],b[2]);
+            assert ValidState(b[2]);
+            assert (OperandContents(b[1],z).val <= 2147483647) ==> OperandContents(b[2],result).val == 1;
+    //
+            assert ValidOperand(b[2],result);
+            assert ValidInstruction(b[2],RET(result));
+            assert NextStep(b[2],b[3],Step.evalInsStep(RET(result)));
+            assert StateNext(b[2],b[3]);
+            assert OperandContents(b[2],result) == OperandContents(b[3],result);
+
+            assert ValidState(b[3]);
+
+            // LAST STEP
+            assert b[3] == b[4];
+            assert ValidState(b[4]);
+            assert NextStep(b[3],b[4],Step.stutterStep());
+            assert StateNext(b[3],b[4]);
+            
+            // Properties
+            assert ValidBehaviorNonTrivial(b);
+            assert BehaviorEvalsCode(c,b);
+            assert OperandContents(s,input).val < 2 ==> OperandContents(b[2],result).val == 1;
+            assert OperandContents(s,input).val == 2 ==> OperandContents(last(b),result).val == 0;
+            assert ValidOperand(last(b),z);
+            assert OperandContents(s,input).val > 0 ==> OperandContents(b[1],z).val > 0;
+            assert |b| == 5;
+            assert Out(OperandContents(b[2],result)) in behaviorOutput(b);
+            assert (OperandContents(b[2],result) == (Int(1,IntType(1,false)))) || (OperandContents(b[2],result) == (Int(0,IntType(1,false))));
+
+            assert behaviorOutput(b) == [Nil,Nil,Nil,Out(OperandContents(b[2],result)),Out(OperandContents(b[2],result))];
+
+            assert OperandContents(s,input).val == 2 ==>( exists result:operand :: 
+                                                            (&& ValidState(last(b))
+                                                            && result.LV?
+                                                            && result.l in last(b).lvs
+                                                            && ValidOperand(last(b),result)
+                                                            && OperandContents(last(b),result).Int?
+                                                            && OperandContents(last(b),result).val == 0));
+
+        }
+
+    lemma validInputPatchImpliesBehavior(s:state)
+        requires ValidState(s);
+        ensures forall input :: validInput(s,input) ==> (exists b :: BehaviorEvalsCode(codePatch(input),b) && b[0] == s)
+    {
+        forall input | validInput(s,input)
+            ensures exists b :: BehaviorEvalsCode(codePatch(input),b) && b[0] == s
+        {
+            var b := unwrapPatchBehaviors(s,input);
+            assert exists b' :: BehaviorEvalsCode(codePatch(input),b') && b'[0] == s;
+        }
+    }
+
+    lemma validInputVulnImpliesBehavior(s:state)
+        requires ValidState(s);
+        ensures forall input :: validInput(s,input) ==> (exists b :: BehaviorEvalsCode(codeVuln(input),b) && b[0] == s)
+    {
+        forall input | validInput(s,input)
+            ensures exists b :: BehaviorEvalsCode(codeVuln(input),b) && b[0] == s
+        {
+            var b := unwrapVulnBehaviors(s,input);
+            assert exists b' :: BehaviorEvalsCode(codeVuln(input),b') && b'[0] == s;
+        }
+    }
+
+    predicate nonTrivialBehaviorPreconditions(s:state,vulnBehaviors:seq<behavior>,patchBehaviors:seq<behavior>)
+    {
+        && ValidState(s)
+        && nonTrivialBehaviorPreconditionsVuln(s,vulnBehaviors)
+        && nonTrivialBehaviorPreconditionsPatch(s,patchBehaviors)
+        && |vulnBehaviors| >= |patchBehaviors|
+      
+    }
+
+    predicate nonTrivialBehaviorPreconditionsPatch(s:state,patchBehaviors:seq<behavior>)
+        requires ValidState(s)
+    {   
+        (forall b :: b in patchBehaviors <==> (exists input :: validInput(s,input) && BehaviorEvalsCode(codePatch(input),b) && b[0] == s))
+    }
+    
+    predicate nonTrivialBehaviorPreconditionsVuln(s:state,vulnBehaviors:seq<behavior>)
+        requires ValidState(s)
+    {
+        (forall b :: b in vulnBehaviors <==> (exists input :: validInput(s,input) && BehaviorEvalsCode(codeVuln(input),b) && b[0] == s))
+    }
+
+    predicate validPatchBehavior(b:behavior)
+    {
+        exists input :: BehaviorEvalsCode(codePatch(input),b) && |b| > 0 && ValidState(b[0]) && validInput(b[0],input)
+    }
+
+    predicate validVulnBehavior(b:behavior)
+    {
+        exists input :: BehaviorEvalsCode(codeVuln(input),b) && ValidBehaviorNonTrivial(b)
+    }
+
+}
