Dafny/examples/BasicBug/simpleBugGeneral.i.dfy
@@ -1,0 +1,72 @@
+include "../../LLVM/llvmREFACTOR.i.dfy"
+include "../../LLVM/types.dfy"
+include "../../Libraries/Seqs.s.dfy"
+
+module simpleBugGeneral{
+    import opened LLVM_defRE
+    import opened types
+    import opened Collections__Seqs_s
+
+        // benignPatch: "The patch does not add any NEW behaviors"
+    predicate benignPatch(a:seq<behavior>,b:seq<behavior>)
+    {
+        var aOut := allBehaviorOutput(a);
+        var bOut := allBehaviorOutput(b);
+        forall p :: p in bOut ==> p in aOut
+
+    }
+
+
+// Describes/Excludes 'bad' behaviors in the Unpatched Code (ie preBehaviors)
+    predicate RemovedBehaviors(b:behavior)
+    {
+
+        && ValidBehaviorNonTrivial(b)
+        && ValidState(last(b))
+        && (exists result:LocalVar :: (result in last(b).lvs 
+                                    && ValidOperand(last(b),LV(result))
+                                    && OperandContents(last(b),LV(result)).Int?
+                                    && OperandContents(last(b),LV(result)).val == 0))
+        // && exists s:state :: (&& s in b 
+        //                       && ValidState(s)
+        //                       && ValidOperand(s,result)
+        //                       && OperandContents(s,result).Int?
+        //                       && OperandContents(s,result).val == 0)
+    }
+    predicate RemovedBehaviorsUpdated(b:behavior)
+    {
+        // var result := LV("result"); 
+        && ValidBehaviorNonTrivial(b)
+        && exists s:state,result:operand :: (&& s in b
+                                            && last(b) == s 
+                                            && ValidState(s)
+                                            && result.LV?
+                                            && result.l in s.lvs
+                                            && ValidOperand(s,result)
+                                            && OperandContents(s,result).Int?
+                                            && OperandContents(s,result).val == 0)
+    }
+
+    predicate MiniSpec(b:behavior)
+    {
+        RemovedBehaviorsUpdated(b)
+    }
+
+    // successfulPatch: "The patch prunes the BAD (defined by MiniSpec) behaviors"
+    predicate successfulPatch(b:seq<behavior>)
+    {
+        forall p :: MiniSpec(p) ==> !(p in b)
+    }
+
+
+    
+
+
+   
+
+   
+
+    
+
+
+}
