Dafny/examples/BasicBug/simpleBugProperties.i.dfy
@@ -1,0 +1,79 @@
+include "simpleBugBenignLemmas.i.dfy"
+include "simpleBugCode.i.dfy"
+include "../../LLVM/llvmREFACTOR.i.dfy"
+include "../../LLVM/types.dfy"
+include "simpleBugGeneral.i.dfy"
+include "../../Libraries/Seqs.s.dfy"
+
+
+module simpleBugProperties{
+    import opened simpleBugBenignLemmas
+    import opened simpleBugCode
+    import opened LLVM_defRE
+    import opened types
+    import opened simpleBugGeneral
+    import opened Collections__Seqs_s
+
+
+
+
+
+
+///////////////////////////////
+
+
+    lemma patchIsBenign(s:state,vulnBehaviors:seq<behavior>,patchBehaviors:seq<behavior>)
+        requires nonTrivialBehaviorPreconditions(s,vulnBehaviors,patchBehaviors)
+        ensures benignPatch(vulnBehaviors,patchBehaviors)
+    {
+        var vulnOut := allBehaviorOutput(vulnBehaviors);
+        var patchOut :=  allBehaviorOutput(patchBehaviors);
+        if (|patchBehaviors| == 0){
+            patchIsBenignTrivial(s,vulnBehaviors,patchBehaviors,vulnOut,patchOut);
+            assert forall p :: p in patchOut ==> p in vulnOut;
+        }else{
+            assert |patchBehaviors| > 0;
+            patchIsBenignNonTrivial(s,vulnBehaviors,patchBehaviors,vulnOut,patchOut);
+            assert forall p :: p in patchOut ==> p in vulnOut;
+        }
+    }
+
+
+//  predicate successfulPatch(b:seq<behavior>)
+//     {
+//         forall p :: MiniSpec(p) ==> !(p in b)
+//     }
+
+ lemma patchIssuccessful(s:state,patchBehaviors:seq<behavior>)
+        requires ValidState(s);
+        requires nonTrivialBehaviorPreconditionsPatch(s,patchBehaviors)
+        // ensures benignPatch(vulnBehaviors,patchBehaviors)
+    {    
+        var result := LV("result");
+         if (|patchBehaviors| == 0){
+             assert forall p :: MiniSpec(p) ==> !(p in patchBehaviors);
+         } else {
+             assert |patchBehaviors| > 0;
+             forall p | p in patchBehaviors
+                {  
+                    var input :| BehaviorEvalsCode(codePatch(input),p) && |p| > 0 && validInput(p[0],input);
+                    var b' := unwrapPatchBehaviors(s,input);
+                    // assert ValidOperand(last(p),result);
+                    // assert !RemovedBehaviorsUpdated(p);
+                    assert forall q :: MiniSpec(q) ==> RemovedBehaviors(q);
+                    assert forall q :: MiniSpec(q) ==> (exists s:state,result:operand :: (&& s in q
+                                                                                            && last(q) == s 
+                                                                                            && ValidState(s)
+                                                                                            && result.LV?
+                                                                                            && result.l in s.lvs
+                                                                                            && ValidOperand(s,result)
+                                                                                            && OperandContents(s,result).Int?
+                                                                                            && OperandContents(s,result).val == 0));
+                }
+                
+                // assert forall p :: MiniSpec(p) ==> !(p in patchBehaviors);
+             }
+         }
+    
+
+}
