Dafny/examples/BasicBug/simpleBugSuccessfulLemmas.i.dfy
@@ -1,0 +1,69 @@
+include "simpleBugCode.i.dfy"
+include "simpleBugGeneral.i.dfy"
+include "../../LLVM/llvmREFACTOR.i.dfy"
+include "../../LLVM/types.dfy"
+
+module simpleBugBenignLemmas{
+    import opened simpleBugCode
+    import opened simpleBugGeneral
+    import opened LLVM_defRE
+    import opened types
+
+lemma possibleVulnOutputs(s:state, b:behavior) 
+        requires ValidState(s);
+        requires |b| > 0;
+        requires b[0] == s;
+        requires s.o.Nil?;
+
+        ensures  forall input :: (validInput(s,input) && OperandContents(s,input).val < 2 && BehaviorEvalsCode(codeVuln(input),b)) 
+                                  ==> (behaviorOutput(b) == [Nil,Nil,Nil,Out((Int(1,IntType(1,false)))),Out((Int(1,IntType(1,false))))]);
+        ensures  forall input :: (validInput(s,input) && OperandContents(s,input).val >= 2 && BehaviorEvalsCode(codeVuln(input),b)) 
+                                  ==> (behaviorOutput(b) == [Nil,Nil,Nil,Out((Int(0,IntType(1,false)))),Out((Int(0,IntType(1,false))))]);
+    {
+        var inputWitness := D(Int(1,IntType(4,false)));
+        assert validInput(s,inputWitness);
+        forall input | validInput(s,input) && OperandContents(s,input).val < 2 && BehaviorEvalsCode(codeVuln(input),b)
+            ensures (behaviorOutput(b) == [Nil,Nil,Nil,Out((Int(1,IntType(1,false)))),Out((Int(1,IntType(1,false))))]);
+        {
+            var input :| validInput(s,input) && OperandContents(s,input).val < 2 && BehaviorEvalsCode(codeVuln(input),b);
+            var b' := unwrapVulnBehaviors(s,input);
+        }
+        forall input | validInput(s,input) && OperandContents(s,input).val >= 2 && BehaviorEvalsCode(codeVuln(input),b)
+            ensures (behaviorOutput(b) == [Nil,Nil,Nil,Out((Int(0,IntType(1,false)))),Out((Int(0,IntType(1,false))))]);
+        {
+            var input :| validInput(s,input) && OperandContents(s,input).val >= 2 && BehaviorEvalsCode(codeVuln(input),b);
+            var b' := unwrapVulnBehaviors(s,input);
+        }
+     
+    }
+
+    lemma possiblePatchOutputs(s:state, b:behavior) 
+        requires ValidState(s);
+        requires |b| > 0;
+        requires b[0] == s;
+        requires s.o.Nil?;
+
+        ensures  forall input :: (validInput(s,input) && BehaviorEvalsCode(codeVuln(input),b)) 
+                                  ==> (behaviorOutput(b) == [Nil,Nil,Nil,Out((Int(1,IntType(1,false)))),Out((Int(1,IntType(1,false))))]);
+        // ensures  forall input :: (validInput(s,input) && OperandContents(s,input).val >= 2 && BehaviorEvalsCode(codeVuln(input),b)) 
+        //                           ==> (behaviorOutput(b) == [Nil,Nil,Nil,Out((Int(0,IntType(1,false)))),Out((Int(0,IntType(1,false))))]);
+    {
+        var inputWitness := D(Int(1,IntType(4,false)));
+        assert validInput(s,inputWitness);
+        forall input | validInput(s,input)  && BehaviorEvalsCode(codeVuln(input),b)
+            ensures (behaviorOutput(b) == [Nil,Nil,Nil,Out((Int(1,IntType(1,false)))),Out((Int(1,IntType(1,false))))]);
+        {
+            var input :| validInput(s,input) && BehaviorEvalsCode(codeVuln(input),b);
+            var b' := unwrapPatchBehaviors(s,input);
+        }
+        // forall input | validInput(s,input) && OperandContents(s,input).val >= 2 && BehaviorEvalsCode(codeVuln(input),b)
+        //     ensures (behaviorOutput(b) == [Nil,Nil,Nil,Out((Int(0,IntType(1,false)))),Out((Int(0,IntType(1,false))))]);
+        // {
+        //     var input :| validInput(s,input) && OperandContents(s,input).val >= 2 && BehaviorEvalsCode(codeVuln(input),b);
+        //     var b' := unwrapVulnBehaviors(s,input);
+        // }
+     
+    }
+
+
+}
